\begin{enumerate}[label=\thechapter.\arabic*,ref=\thechapter.\theenumi]
\numberwithin{equation}{enumi}
\numberwithin{figure}{enumi}
\numberwithin{table}{enumi}
\item The Differentiation in frequency domain is as follows\\
        Let x(t) be a signal such that,
    \begin{align}
        x\brak{t}&\xleftrightarrow{\text{F.T}} X\brak{\omega}\\
        X\brak{\omega}&=\int_{t=-\infty}^{\infty}x\brak{t}e^{-j\omega t}dt\\
        \frac{d}{d\omega}X\brak{\omega}&=\int_{t=-\infty}^{\infty}x\brak{t}\brak{-jt}e^{-j\omega t}dt\\
        j\frac{d}{d\omega}X\brak{\omega}&=\int_{t=-\infty}^{\infty}tx\brak{t}e^{-j\omega t}dt\\
        tx\brak{t}&\xleftrightarrow{\text{F.T}} j\frac{d}{d\omega}X\brak{\omega}\label{eq:Differentiation-property}
    \end{align}
\item The duality property is as follows\\
    From inverse Fourier transform we get,
    \begin{align}
        x\brak{t}&=\frac{1}{2\pi}\int_{-\infty}^{\infty}X\brak{\omega}e^{j\omega t}d\omega
    \end{align}
    Replacing t by -t and multiplying 2$\pi$ on both sides we get,
    \begin{align}
        2\pi x\brak{-t}&=\int_{-\infty}^{\infty}X\brak{\omega}e^{-j\omega t}d\omega\\
        X\brak{t}&\xleftrightarrow{\text{F.T}} 2\pi x\brak{-\omega}\label{eq:Duality-property}
    \end{align}
    
\item Complex Fourier Series	\\
\begin{align}
	x(t) &= \sum_{n=-\infty}^{\infty} c_{n}e^{j2\pi nft}
	\label{eq:compfs}
\end{align}
where $c_{n}$ is the exponential fourier coefficient.
\begin{align}
        c_{n} &= \frac{1}{T} \int_{0}^{T} x(t) e^{-j2\pi nft} \, dt
\end{align}
where $T$ is the time period of function $x(t)$.
\item Trigonometric Fourier Series	\\
\begin{align}
	e^{j2\pi nft} = cos(2\pi nft ) + j sin(2\pi nft)
	\label{eq:expfs}
\end{align}
Substituting \eqref{eq:expfs} in \eqref{eq:compfs}
\begin{align}
	 x(t) &= \sum_{n=-\infty}^{\infty} c_{n} \brak{\cos(2\pi nft) + j \sin(2\pi nft)}\\
	      &= a_0 + \sum_{n=1}^{\infty} \brak{a_{n} \cos(2\pi nft)} + \brak{b_{n} \sin(2\pi nft)}
\end{align}
where $a_0, a_{n}$ and $b_{n}$ are trigonometric fourier series.
\begin{align}
          a_{0} &= c_{0}\\
                &=\frac{1}{T} \int_{0}^{T} x(t) \, dt\\
          a_{n} &= 2Re(c_{n})\\
                &=\frac{2}{T} \int_{0}^{T} x(t)\cos(2\pi nft) \, dt\\
          b_{n} &= -2Im(c_{n})\\
                &= \frac{2}{T} \int_{0}^{T} x(t)\sin(2\pi nft) \, dt
\end{align}

\item Peridicity of Fourier coefficients\\
For a signal $x[n] = \sum_{k=0}^{N-1}a_ke^{j\brak{\frac{2kn\pi}{N}}}$, defining $X[k] = Na_k$.
\begin{align}
x[n] &= \frac{1}{N}\sum_{k=0}^{N-1}X[k]e^{j\brak{\frac{2kn\pi}{N}}}\\
\sum_{n=0}^{N-1}x[n]e^{-j\brak{\frac{2rn\pi}{N}}} &= \sum_{n=0}^{N-1}\frac{1}{N}\sum_{k=0}^{N-1}X[k]e^{j\brak{\frac{2kn\pi}{N}}}e^{-j\brak{\frac{2rn\pi}{N}}}\\
&= \sum_{k=0}^{N-1}X[k]\sum_{n=0}^{N-1}\frac{1}{N}e^{j\brak{\frac{2\brak{k-r}n\pi}{N}}}\\
\sum_{n=0}^{N-1}\frac{1}{N}e^{j\brak{\frac{2\brak{k-r}n\pi}{N}}}&=\begin{cases}
1 & k-r=mN, m \in \mathbb{Z}\\
0 & \text{ otherwise}
\end{cases}\\
\implies X[k] &= \sum_{n=0}^{N-1}x[n]e^{-j\brak{\frac{2kn\pi}{N}}} \label{X[k]_F_coeff}
\end{align}
If $x[n] = x[n+rN],r \in \mathbb{Z}$, from \eqref{X[k]_F_coeff},
\begin{align}
X[k+rN] &= \sum_{n=0}^{N-1}x[n]e^{-j\brak{\frac{2\brak{k+rN}n\pi}{N}}}\\
&= \sum_{n=0}^{N-1}x[n]e^{-j\brak{\frac{2kn\pi}{N}}}e^{-j\brak{2rn\pi}}\\
&= \sum_{n=0}^{N-1}x[n]e^{-j\brak{\frac{2kn\pi}{N}}}\\
&= X[k]\\
\implies a_k &= a_{k+rN},r \in \mathbb{Z} \label{a_k=a_{k+rN}}
\end{align}
\end{enumerate}
